

## Lab-2

Aim: Convert a given infix expression to Postfix and display it. Expression consists of binary operators (+, -, \*, /)

Code:

```
#include <stdio.h>
#include <ctype.h>
#include <string.h>

#define MAX
stack [MAX], postfix [MAX]
infix
top = -1
```

function precedence (op):

```
if op is '+' or '-'
    return 1
else if op is '*' or '/'
    return 2
else if op is '^'
    return 3
else if op is '('
    return 0
```

function associativity (op):

```
if op is '^'
    return 1 (Right to left)
else
    return 0 (Left to right)
```

function push (ch):

```
if top == MAX-1
    print 'Stack overflow'
    return
stack[++top] = ch
```

```
function pop():
```

```
    if top == -1
```

```
        print 'stack underflow'
```

```
    return stack[top--]
```

```
function peek():
```

```
    if top == -1
```

```
        print 'stack is empty'
```

```
    return stack[top]
```

```
function infixToPostfix(char infix[], char postfix[]):
```

```
    for (int i = 0; i <
```

```
        int i, p = 0
```

```
        char c
```

```
        for (int i = 0; i < strlen(infix[i]); i++)
```

```
            c = infix[i]
```

```
            if (infix[i] is operand)
```

```
                push into postfix[p]
```

```
            else if (c == '(')
```

```
                push into stack
```

```
            else if (c == ')')
```

```
                while (peek() != '(')
```

```
                    postfix[k] =
```

```
                    postfix[p++] = pop()
```

```
            else
```

```
                while (top != 1 and precedence(peek()) >=
```

```
                    (precedence(c) or precedence(peek()) ==
```

```
                    precedence(c) and associativity == 0)
```

```
                postfix[p++] = pop()
```

```
            }  
        }  
    }  
    pop()
```



function main ( ) :

input infix [ ]

# infixToPostfix [infix, postfix]

print (postfix [ ])

return

Output :

I. Enter a valid parenthesized infix expression:  $(a+b*c)$

Postfix expression:  $abc*+$

II. Enter a valid parenthesized infix expression:  $((a+b)*c)$

Postfix expression:  $ab+c*$

III. Enter a valid parenthesized infix expression:  $(a^b(c))$

Postfix expression:  $abc^{\wedge}$

IV. Enter a valid parenthesized infix expression:  $((a+b)*(c-d))$

Postfix expression:  $ab+cd-*$

V. Enter a valid parenthesized infix expression:  $(a+b*c-d/e)$

Postfix expression:  $abc*+de/-$

Wohh!

```
Enter a valid parenthesized infix expression : (a+b*c)
Postfix expression : abc*+
Process returned 0 (0x0)   execution time : 3.245 s
```

```
Enter a valid parenthesized infix expression : ((a+b)*c)
Postfix expression : ab+c*
Process returned 0 (0x0)   execution time : 9.120 s
```

```
Enter a valid parenthesized infix expression : (a^(b^c))
Postfix expression : abc^^
Process returned 0 (0x0)   execution time : 2.367 s
```

```
Enter a valid parenthesized infix expression : ((a+b)*(c-d))
Postfix expression : ab+cd-*
Process returned 0 (0x0)   execution time : 2.379 s
```

```
Enter a valid parenthesized infix expression : (a+b*c-d/e)
Postfix expression : abc*+de/-
Process returned 0 (0x0)   execution time : 2.220 s
```